

数字电子技术第一次作业

17 $(100)_{10} = (64)_{16} = (1100100)_2$ $(127)_{10} = (7F)_{16} = (1111111)_2$
 $(255)_{10} = (FF)_{16} = (11111111)_2$ $(165)_{10} = (108)_{16} = (10000101)_2$
 $(50375)_{10} = (326)_{16} = (110010011)_2$

18 $(1011)_2 = (B)_{16} = (11)_{10}$ $(10000000)_2 = (80)_{16} = (128)_{10}$
 $(11001011)_2 = (196)_{16} = (25375)_{10}$ $(10100101)_2 = (A5)_{16} = (103125)_{10}$

19 $(AF3C)_{16} = (1010111100111100)_2 = (127474)_8$ $(0F)_{16} = (00001111)_2 = (017)_8$
 $(80)_{16} = (10000000)_2 = (200)_8$ $(3BD8)_{16} = (001110111011)_2 = (16758)_{10}$

110
 $(+1011)_2$ 原码: 01011 反码: 01011 补码: 01011
 $(+00110)_2$ 原码: 000110 反码: 000110 补码: 000110
 $(-1101)_2$ 原码: 11101 反码: 10010 补码: 10011
 $(-00101)_2$ 原码: 100101 反码: 111010 补码: 111011

111 (1) 证: $A \oplus 1 = \bar{A}$

A	$A \oplus 1$	\bar{A}
0	1	1
1	0	0

 (2) 证: $A \oplus 0 = A$

A	$A \oplus 0$	A
0	0	0
1	1	1

(3) 证: $A(B \oplus C) = AB \oplus AC$

A	B	C	AC	AB	$B \oplus C$	$A(B \oplus C)$	$AB \oplus AC$
0	0	0	0	0	0	0	0
0	0	1	0	0	1	0	0
0	1	0	0	0	1	0	0
0	1	1	0	1	0	0	0
1	0	0	0	0	0	0	0
1	0	1	0	0	1	0	0
1	1	0	0	1	1	1	1
1	1	1	1	1	0	0	0

$$(4) A \oplus \bar{B} = \overline{A \oplus B}$$

A	B	\bar{B}	$A \oplus \bar{B}$	$A \oplus B$	$\overline{A \oplus B}$
0	0	1	1	0	1
0	1	0	0	1	0
1	0	1	0	1	0
1	1	0	1	0	1

$$(5) (A \oplus B) \oplus C = A \oplus (B \oplus C)$$

A	B	C	$A \oplus B$	$(A \oplus B) \oplus C$	$B \oplus C$	$A \oplus (B \oplus C)$
0	0	0	0	0	0	0
0	0	1	0	1	1	1
0	1	0	1	0	1	0
0	1	1	1	1	0	1
1	0	0	1	0	0	0
1	0	1	1	1	1	1
1	1	0	0	0	1	0
1	1	1	0	1	0	1

$$112 (1) Y = \bar{A}BC + AC + B\bar{C}$$

$$= \sum_m (2, 3, 5, 6, 7)$$

$$(2) Y = \overline{ABC}D + BCD + AC$$

$$= \sum_m (7, 9, 10, 11, 14, 15)$$

$$(3) Y = AB + BC + ACD$$

$$= \sum_m (6, 7, 11, 12, 13, 14, 15)$$

$$(4) Y = AB + \overline{BC(C + \bar{D})} \quad (\text{德摩根律化简})$$

$$= AB + \overline{BC}(\bar{C} + \bar{D}) = AB + \bar{B}\bar{C} + \bar{C}\bar{D}$$

$$= \sum_m (3, 6, 7, 11, 12, 13, 14, 15)$$

$$113 (1) Y = (A+B)(\bar{A}+\bar{B}+\bar{C})$$

$$= (A+B+C)(A+B+\bar{C})(\bar{A}+\bar{B}+\bar{C}) = \prod M(0, 1, 7)$$

$$(2) Y = A\bar{B} + \bar{A}C = (A+B+C)(A+\bar{B}+C)(\bar{A}+\bar{B}+C)(\bar{A}+\bar{B}+\bar{C}) = \prod M(0, 2, 6, 7)$$

$$(3) Y = BC\bar{D} + \bar{A}D + C \quad \rightarrow = \prod M(0, 4, 8, 9, 12, 13)$$

$$= (A+B+C+D)(\bar{A}+\bar{B}+C+D)(A+\bar{B}+C+D)(\bar{A}+\bar{B}+C+D)(\bar{A}+\bar{B}+C+\bar{D})$$

$$(4) Y = \sum (m_1, m_2, m_4, m_6, m_7)$$

$$= (\bar{A}+\bar{B}+\bar{C})(\bar{A}+B+C)(A+\bar{B}+C) = \prod M(0, 3, 5)$$

$$115 (1) Y = \bar{A}\bar{B}C + \bar{A}B\bar{C} + A\bar{B}\bar{C} + ABC$$

$$(2) Z = \bar{M}\bar{N}PQ + \bar{M}NP\bar{Q} + \bar{M}NPQ + MNP\bar{Q} + MN\bar{P}\bar{Q} + MN\bar{P}Q + MNPQ + MN\bar{P}Q$$

$$117 (1) Y = (A+B)(\bar{A}+C) + BC$$

$$\bar{Y} = (\bar{A}\bar{B} + \bar{A}\bar{C}) \cdot \bar{B}\bar{C} = \bar{A}\bar{B}\bar{C} + \bar{A}\bar{B}\bar{C}$$

$$= \bar{B}\bar{C}$$

$$(2) Y = (\overline{A+C}) \cdot \overline{AD + \bar{B}C + A\bar{B}D}$$

$$\bar{Y} = (\bar{A}\bar{C}) \cdot (\bar{B}+\bar{D}) + (\bar{A}+\bar{D}) \cdot (\bar{B}+\bar{C}) \cdot (\bar{A}+B+\bar{D})$$

$$= ((A+C)(\bar{B}+\bar{D})) + ((AD + \bar{B}C) \cdot (\bar{A}+B+\bar{D}))$$

$$= A + \bar{B}C + \bar{C}\bar{D}$$

$$(3) Y = [(A+D)\overline{AC} + \overline{ABD}](\overline{A+C+BD})$$

$$\begin{aligned}\overline{Y} &= [(\overline{A\overline{D} + (\overline{A+C})}) (A+\overline{B+D})] + (\overline{AC})(\overline{B+D}) \\ &= [(\overline{AC + AD + CD}) (A+\overline{B+D})] + (A+C)(\overline{B+D}) \\ &= A\overline{B} + A\overline{C} + A\overline{D} + \overline{B}C + \overline{C}D + \overline{C}D + D\overline{A} + \overline{A}\overline{B}D\end{aligned}$$

$$(4) Y = (\overline{A \oplus C})(\overline{B+D})(\overline{BD+AC}) = (\overline{AC+\overline{AC}})(\overline{B+D})(\overline{BD+AC})$$

$$\begin{aligned}\overline{Y} &= (\overline{A+C})(\overline{A+C}) + \overline{BD} + (\overline{B+D})(\overline{A+C}) = (\overline{AC+\overline{AC}})(\overline{B+D}) + (\overline{B+D})(\overline{A+C}) \\ &= A\overline{B}C + \overline{A}BC + \overline{A}\overline{B} + \overline{A}\overline{D} + \overline{B}C + \overline{C}D\end{aligned}$$

$$118 (1) Y = A(B+C) + \overline{BC}A\overline{B}$$

$$(2) Y = (A+C)(\overline{B+D}) + \overline{BC+D}AD$$

$$\therefore Y' = (A+BC)(B+C + \overline{A+B})$$

$$Y' = (AC + \overline{BD})((\overline{B+C})D + A+D)$$

$$(3) Y = \overline{AB + \overline{ACD}} + \overline{B+C}(A+\overline{B+D})$$

$$(4) Y = \overline{(A+B)(\overline{C+D})(A+B+C)} + (\overline{A+B})C$$

$$Y' = [(\overline{A+B})(\overline{A+C}+D)] \cdot (\overline{BC} + A\overline{BD})$$

$$= (\overline{AB} + \overline{CD} + A\overline{BC})(\overline{A+B}+C)$$

$$119 (1) Y = A\overline{B} + B + \overline{A}C = A+B+\overline{A}C = A+B+C$$

$$(2) Y = \overline{ABC} + \overline{A}\overline{B} = (A+\overline{B}+\overline{C}) + (\overline{A+B}) = 1$$

$$\begin{aligned}(3) Y &= \overline{A\overline{B}CD} + \overline{ABD} + \overline{ACD} = \overline{A\overline{B}CD} + \overline{ABCD} + \overline{A\overline{B}CD} + \overline{ACD} \\ &= ACD + A\overline{C}D + AD\overline{B}C = AD + AD\overline{B}C = AD\end{aligned}$$

$$\begin{aligned}(4) Y &= \overline{AC} + \overline{ABC} + \overline{ACD} + \overline{CD} = \overline{AC} + \overline{ABC} + \overline{ACD} + \overline{ACD} + \overline{ACD} \\ &= \overline{AC} + \overline{AC} + \overline{ABC} + \overline{ACD} = \overline{AC} + \overline{AC} + \overline{ACD} = A + \overline{ACD} = A + \overline{CD}\end{aligned}$$

$$(5) Y = A\overline{B}(\overline{ACD} + \overline{AD+BC})(\overline{A+B}) = A\overline{B}\overline{A\overline{B}}(\overline{ACD} + \overline{AD+BC}) = 0$$

$$(6) Y = (\overline{A+B})(\overline{B+C})(\overline{C+D})(\overline{D+A}) = \overline{A\overline{B}C\overline{D}} + \overline{ABCD}$$

$$\begin{aligned}(7) Y &= AC(\overline{CD} + \overline{AB}) + BC(\overline{B+AD} + \overline{CE}) \\ &= BC \cdot ((\overline{B+AD})(\overline{C+E})) = BCAD\overline{E} = ABCD\overline{E}\end{aligned}$$

$$\begin{aligned}(8) Y &= \overline{A\overline{B}C\overline{D}} + \overline{A\overline{B}C\overline{D}} + \overline{B\overline{C}D} = \overline{A\overline{B}C\overline{D}} + \overline{B\overline{C}D} + A \\ &= A + \overline{B\overline{C}D} + B + \overline{C} + D = A+B+\overline{C}+D\end{aligned}$$